Trace semantics of Nimp

examples/Nimp.v
@@ -1,7 +1,7 @@
 (* A nondeterministic Imp *)
 
 From Coq Require Import
-     Relations.
+     List Relations.
 
 From Paco Require Import paco2.
 
@@ -15,6 +15,7 @@ Inductive com : Type :=
 | seq : com -> com -> com
 .
 
+(* note(LY): I think ExtLib put this level too high *)
 Infix ";;" := seq (at level 100, right associativity) : com_scope.
 Delimit Scope com_scope with com.
 Open Scope com_scope.
@@ -102,6 +103,209 @@ Proof.
 Qed.
 
 End Labeled.
+
+(* Set of traces semantics *)
+Module Traces.
+Import ListNotations.
+
+Inductive dir := Left | Right.
+
+Module Naive.
+
+Definition trace : Type := list dir.
+
+(* Sets of traces *)
+Definition trace_set : Type := trace -> Prop.
+
+(* One trace, the empty trace. *)
+Definition empty_trace : trace_set :=
+  fun tr => tr = [].
+
+Definition one : dir -> trace_set :=
+  fun d tr => tr = [d].
+
+Definition seq : trace_set -> trace_set -> trace_set :=
+  fun P1 P2 tr =>
+    exists tr1 tr2, tr = tr1 ++ tr2 /\ P1 tr1 /\ P2 tr2.
+
+Definition or : trace_set -> trace_set -> trace_set :=
+  fun P1 P2 tr => P1 tr \/ P2 tr.
+
+(* star P tr <->
+   exists tr1 ... trn,
+     (tr = tr1 ++ ... ++ trn) /\
+     P tr1 /\ ... /\ P trn *)
+Inductive star (P : trace_set) : trace_set :=
+| star_0 : star P []
+| star_1 tr1 tr2 : P tr1 -> star P tr2 -> star P (tr1 ++ tr2)
+.
+
+Fixpoint eval (c : com) : trace_set :=
+  match c with
+  | loop c' => seq (star (seq (one Right) (eval c'))) (one Left)
+  | choose c1 c2 => or (eval c1) (eval c2)
+  | skip => empty_trace
+  | (c1 ;; c2) => seq (eval c1) (eval c2)
+  end.
+
+(* The problem with this definition is it only captures traces of
+   complete but finite executions. *)
+
+End Naive.
+
+Module PrefixClosed.
+(* To define "prefix closed sets of traces", one issue is that in
+   [seq P1 P2] we have to be careful to append traces of [P2] only
+   to "complete" traces of [P1]. So we need to enrich the type of
+   traces. *)
+
+(* Explicit marker for termination. *)
+Inductive fin := Done | More.
+
+Definition le_fin (f1 f2 : fin) : Prop :=
+  match f1, f2 with
+  | Done, More => False
+  | _, _ => True
+  end.
+
+Delimit Scope fin_scope with fin.
+Infix "<=" := le_fin : fin_scope.
+
+Lemma Done_max f : (f <= Done)%fin.
+Proof. destruct f; constructor. Qed.
+
+Lemma More_min  f : (More <= f)%fin.
+Proof. constructor. Qed.
+
+Hint Resolve Done_max More_min.
+
+Definition trace : Type := list dir * fin.
+
+Inductive prefix : trace -> trace -> Prop :=
+| prefix_cons d tr1 f1 tr2 f2 :
+    prefix (tr1, f1) (tr2, f2) -> prefix (d :: tr1, f1) (d :: tr2, f2)
+| prefix_nil f1 tr2 f2 :
+    (f1 <= f2)%fin ->
+    prefix (nil, f1) (tr2, f2)
+.
+
+Lemma prefix_trans tr0 tr1 tr2 :
+  prefix tr0 tr1 -> prefix tr1 tr2 -> prefix tr0 tr2.
+Proof.
+Admitted.
+
+Lemma le_fin_prefix tr f1 f2 : (f1 <= f2)%fin -> prefix (tr, f1) (tr, f2).
+Proof.
+  intros.
+  induction tr; constructor; auto.
+Qed.
+
+Lemma prefix_app tr0 f0 tr1 tr2 f12 :
+  prefix (tr0, f0) (tr1 ++ tr2, f12) ->
+  prefix (tr0, f0) (tr1, More) \/
+  exists tr0', tr0 = tr1 ++ tr0' /\ prefix (tr0', f0) (tr2, f12).
+Proof.
+Admitted.
+
+Module Import Core.
+
+(* Sets of traces *)
+Definition trace_set : Type := trace -> Prop.
+
+Definition empty : trace_set := fun _ => False.
+
+Definition empty_trace : trace_set := fun tr =>
+  exists f, tr = ([], f).
+
+Definition one : dir -> trace_set := fun d tr =>
+  prefix tr ([d], Done).
+
+Variant seq (P1 P2 : trace_set) : trace_set :=
+(* A trace of P1, complete or incomplete *)
+| seq_first tr1 f1 : P1 (tr1, f1) -> seq P1 P2 (tr1, f1)
+| seq_both tr1 tr2 f2 : P1 (tr1, Done) -> P2 (tr2, f2) -> seq P1 P2 (tr1 ++ tr2, f2)
+.
+
+Definition or (P1 P2 : trace_set) : trace_set :=
+  fun tr => P1 tr \/ P2 tr.
+
+Inductive star (P : trace_set) : trace_set :=
+| star_end tr f : P (tr, f) -> star P (tr, f)
+| star_continue tr1 tr2 f2 :
+    P (tr1, Done) -> star P (tr2, f2) -> star P (tr1 ++ tr2, f2).
+
+Definition prefix_closed (P : trace -> Prop) :=
+  forall tr1 tr2, P tr2 -> prefix tr1 tr2 -> P tr1.
+
+Lemma prefix_closed_empty : prefix_closed empty.
+Proof. intros ? ? []. Qed.
+
+Lemma prefix_closed_empty_trace : prefix_closed empty_trace.
+Proof.
+  intros tr1 tr2 [] Hprefix.
+  subst; inversion Hprefix.
+  eexists; auto.
+Qed.
+
+Lemma prefix_closed_one d : prefix_closed (one d).
+Proof.
+  intros tr1 tr2 Htr2 Hprefix.
+  inversion Htr2; subst.
+  - inversion Hprefix; subst.
+    + inversion H1; subst.
+      inversion H2; subst.
+      constructor; constructor; auto.
+    + constructor; auto.
+  - inversion Hprefix.
+    constructor; auto.
+Qed.
+
+Lemma prefix_closed_seq P1 P2
+      (H1 : prefix_closed P1) (H2 : prefix_closed P2) :
+  prefix_closed (seq P1 P2).
+Proof.
+  intros [tr1 f1] [tr2 f2] Htr2 Hprefix.
+  inversion Htr2; subst.
+  - eapply seq_first, H1; eauto.
+  - apply prefix_app in Hprefix.
+    destruct Hprefix as [Hprefix | [tr0' [L M]] ].
+    + eapply seq_first, H1; eauto.
+      eapply prefix_trans.
+      * eassumption.
+      * apply le_fin_prefix; auto.
+    + subst.
+      eapply seq_both; auto.
+      eapply H2; eauto.
+Qed.
+
+Lemma prefix_closed_or P1 P2
+      (H1 : prefix_closed P1) (H2 : prefix_closed P2) :
+  prefix_closed (or P1 P2).
+Proof.
+  intros tr1 tr2 [|].
+  - left; eapply H1; eauto.
+  - right; eapply H2; eauto.
+Qed.
+
+Lemma prefix_closed_star P (H : prefix_closed P) :
+  prefix_closed (star P).
+Proof.
+Admitted.
+
+End Core.
+
+(* Prefix-closed sets of traces. *)
+Definition trace_set1 : Type :=
+  { P : trace -> Prop
+  | prefix_closed P }.
+
+End PrefixClosed.
+
+Module Coinductive.
+(* TODO: Define [trace] as a coinductive type. *)
+End Coinductive.
+
+End Traces.
 
 Module Tree.
 
